finally got smn verified with all ADTs

SlowTest/SMN-ADT-ListContLen.dfy
@@ -2,32 +2,43 @@
 // RUN: %diff "%s.expect" "%t"
 
 datatype List<X> = Nil | Cons(head: X, tail: List<X>)
+datatype Nat = Z | S(Nat)
 
 type AbInt(==)
-function method int2adt (n: int) : (r: AbInt)
-// function method adt2int (n: AbInt) : (r: int)
-//   decreases n
-//   ensures n == int2adt(0) ==> r == 0
-//   ensures forall x :: AbAdd(int2adt(1), x) == n ==> r == 1 + adt2int(x)
+function method int2adt (n: int) : (AbInt)
+function method adt2dt (a: AbInt) : Nat
+lemma Props_adt_dt_lt (x: AbInt, y: AbInt)
+  requires AbLt(x, y)
+  ensures adt2dt(x) < adt2dt(y)
 
-predicate AbIsZero (n: AbInt) {n == int2adt(0)}
-predicate AbNonNeg (n: AbInt) { true }
-predicate AbPos (n: AbInt) {AbNonNeg(n) && !AbIsZero(n)}
+predicate AbIsZero (n: AbInt) { n == int2adt(0) }
+predicate AbPos (n: AbInt) { !AbIsZero(n) }
+// predicate AbNonNeg (n: AbInt) { true }
 
 function method AbLt(n: AbInt, m: AbInt) : bool
 function method AbAdd(n: AbInt, m: AbInt) : (r: AbInt)
 function method AbSub(n: AbInt, m: AbInt) : (r: AbInt)
 function method AbDiv2(n: AbInt): (r: AbInt)
   ensures AbLt(AbAdd(r, r), n) || AbAdd(r, r) == n
+function method AbSetLen(s: set<AbInt>) : (l: AbInt)
+lemma SetLen_Props()
+  ensures forall x :: AbSetLen(x) == int2adt(0) <==> x == {}
+  ensures forall x: AbInt :: AbSetLen({x}) == int2adt(1)
+  ensures forall x: AbInt, A: set<AbInt> :: x in A ==> AbSetLen(A) == AbAdd(AbSetLen(A - {x}), int2adt(1))
+  
+  // ensures forall x: AbInt, A, B: set<AbInt> :: x in A && x in B ==> 
+  // ensures forall A: set<AbInt>, B : set<AbInt> :: AbAdd(AbSetLen(A+B), AbSetLen(A*B)) == AbAdd(AbSetLen(A), AbSetLen(B))
+  // ensures forall A: set<AbInt>, B : set<AbInt> :: AbAdd(AbSetLen(A-B), AbSetLen(A*B)) == AbSetLen(A)
+  // ensures forall A: set<AbInt>, B : set<AbInt> :: A !! B ==> AbSetLen(A+B) == AbAdd(AbSetLen(A), AbSetLen(B))
+  // ensures forall A: set<AbInt>, B : set<AbInt> :: AbLt(AbSetLen(A+B), AbAdd(AbSetLen(A), AbSetLen(B))) || AbSetLen(A+B) == AbAdd(AbSetLen(A), AbSetLen(B))
 
 // Set generation: lo <= x < lo+len
 // experiment with more trigger options
 function method AbBoundSet(lo: AbInt, len: AbInt): (S: set<AbInt>)
-  ensures int2adt(|S|) == len
+  ensures AbSetLen(S) == len
   ensures forall x :: (AbLt(lo, x) || lo == x) && AbLt(x, AbAdd(lo, len)) <==> x in S
   // Try not to assign every element with AbAdd()
   // ensures S == set x | 0 <= x < len :: AbAdd(lo, int2adt(x))
-
 
 /* Properties */
 lemma Props_int_pos(a: int)
@@ -35,159 +46,115 @@ lemma Props_int_pos(a: int)
 lemma Props_int_cmp_lt(a: int, b: int) // Lt(a, b)
   ensures AbLt(int2adt(a), int2adt(b))
 
-lemma Props_plus_minus_is_eq ()
-    ensures forall x: AbInt, i, j: int :: AbAdd(AbAdd(x, int2adt(j)), int2adt(i-j)) == AbAdd(x, int2adt(i)) // trigger may loop
-    // ensures forall x: AbInt, i, j, k: int :: k == i - j ==> AbAdd(AbAdd(x, int2adt(j)), int2adt(k)) == AbAdd(x, int2adt(i))
-// Props_plus_minus_is_eq_param(n, len, llen);
-lemma Props_plus_minus_is_eq_param(x: AbInt, i: AbInt, j: AbInt)
-  ensures AbAdd(AbAdd(x, j), AbSub(i, j)) == AbAdd(x, i)
-// Props_eq_less_is_lt_param(s, n, int2adt(llen), int2adt(len));
-lemma Props_eq_less_is_lt_param (x: AbInt, y: AbInt, a: AbInt, b: AbInt)
-  ensures (x == AbAdd(y, a)) && AbLt(a, b) ==> AbLt(x, AbAdd(y, b))
-
-lemma Props ()
-  // Prop_all_leq_zero ()
-  ensures forall x :: AbLt(int2adt(0), x) || x == int2adt(0)
-  // Props_lt_is_not_geq ()
-  ensures forall x, y :: AbLt(x, y) <==> !(AbLt(y, x) || x == y)
-  // Props_lt_addition ()
-  ensures forall x, a, b:: AbLt(a, b) ==> AbLt(AbAdd(x, a), AbAdd(x, b))
-  // Props_lt_transitive ()
-  ensures forall x, y, z :: AbLt(x, y) && AbLt(y, z) ==> AbLt(x, z)
-  // Props_plus_zero ()
-  ensures forall x :: AbAdd(x, int2adt(0)) == AbAdd(int2adt(0), x) == x
-  // Props_eq_less_is_lt ()
-  ensures forall x, y, a, b :: (x == AbAdd(y, a)) && AbLt(a, b) ==> AbLt(x, AbAdd(y, b))
-  // Props_plus_eq_is_lt ()
-  ensures forall x, y, a :: (AbAdd(x, a) == y) && AbNonNeg(a) ==> AbLt(x, y)
-  // Props_plus_lt_is_lt ()
-  ensures forall x, y, a :: AbLt(AbAdd(x, a), y) && AbNonNeg(a) ==> AbLt(x, y)
-  // Props_plus_pos_is_neq ()
-  ensures forall x, a :: AbPos(a) ==> AbAdd(x, a) != x
-  // Props_one_in_bound ()
-  ensures forall a, x :: (AbLt(a, x) || a == x) && (AbLt(x, AbAdd(a, int2adt(1)))) ==> a == x
-  // // Props_plus_minus_is_eq ()
+// lemma Props ()
+//   // Props_all_nonneg ()
+//   ensures forall x :: AbLt(int2adt(0), x) || x == int2adt(0)
+//   // Props_lt_is_not_geq ()
+//   ensures forall x, y :: AbLt(x, y) <==> !(AbLt(y, x) || x == y)
+//   // Props_lt_addition ()
+//   ensures forall x, a, b:: AbLt(a, b) ==> AbLt(AbAdd(x, a), AbAdd(x, b))
+//   // Props_lt_transitive ()
+//   ensures forall x, y, z :: AbLt(x, y) && AbLt(y, z) ==> AbLt(x, z)
+//   // Props_add_identity ()
+//   ensures forall x :: AbAdd(x, int2adt(0)) == AbAdd(int2adt(0), x) == x
+//   // Props_add_less_is_lt ()
+//   ensures forall x, y, a, b :: (x == AbAdd(y, a)) && AbLt(a, b) ==> AbLt(x, AbAdd(y, b))
+//   // Props_add_is_leq ()
+//   ensures forall x, y, a :: (AbAdd(x, a) == y) ==> AbLt(x, y) || x == y
+//   // Props_lt_add_is_lt ()
+//   ensures forall x, y, a :: AbLt(AbAdd(x, a), y) ==> AbLt(x, y)
+//   // Props_add_pos_is_neq ()
+//   ensures forall x, a :: AbPos(a) ==> AbAdd(x, a) != x
+//   // Props_one_in_bound ()
+//   ensures forall a, x :: (AbLt(a, x) || a == x) && (AbLt(x, AbAdd(a, int2adt(1)))) ==> a == x
+  // Props_add_sub_is_add ()
   // ensures forall x: AbInt, i, j: int :: AbAdd(AbAdd(x, int2adt(j)), int2adt(i-j)) == AbAdd(x, int2adt(i)) // trigger may loop
-  ensures forall x: AbInt, i, j, k: int :: k == i - j ==> AbAdd(AbAdd(x, int2adt(j)), int2adt(k)) == AbAdd(x, int2adt(i))
+  // ensures forall x: AbInt, i, j, k: int :: k == i - j ==> AbAdd(AbAdd(x, int2adt(j)), int2adt(k)) == AbAdd(x, int2adt(i))
 
 // duplicate with Props ()
 // Note: if comment out, SMN_Correct doesn't finish.
-// lemma Prop_all_leq_zero ()
-//   ensures forall x :: AbLt(int2adt(0), x) || x == int2adt(0)
-// lemma Props_lt_is_not_geq ()
-//   ensures forall x, y :: AbLt(x, y) <==> !(AbLt(y, x) || x == y)
-// lemma Props_lt_addition () // trigger problem?
-//   ensures forall x, a, b:: AbLt(a, b) ==> AbLt(AbAdd(x, a), AbAdd(x, b))
-// lemma Props_lt_transitive ()
-//   ensures forall x, y, z :: AbLt(x, y) && AbLt(y, z) ==> AbLt(x, z)
-// lemma Props_plus_zero ()
-//   ensures forall x :: AbAdd(x, int2adt(0)) == AbAdd(int2adt(0), x) == x
-// lemma Props_eq_less_is_lt ()
-//   ensures forall x, y, a, b :: (x == AbAdd(y, a)) && AbLt(a, b) ==> AbLt(x, AbAdd(y, b))
-// lemma Props_plus_eq_is_lt ()
-//   ensures forall x, y, a :: (AbAdd(x, a) == y) && AbNonNeg(a) ==> AbLt(x, y)
-// lemma Props_plus_lt_is_lt ()
-//   ensures forall x, y, a :: AbLt(AbAdd(x, a), y) && AbNonNeg(a) ==> AbLt(x, y)
-// lemma Props_plus_pos_is_neq ()
-//   ensures forall x, a :: AbPos(a) ==> AbAdd(x, a) != x
-// lemma Props_one_in_bound ()
-//   ensures forall a, x :: (AbLt(a, x) || a == x) && (AbLt(x, AbAdd(a, int2adt(1)))) ==> a == x
-
-// // Props_eq_less_is_lt_param(s, n, int2adt(llen), int2adt(len));
-// lemma Props_eq_less_is_lt_param (x: AbInt, y: AbInt, a: AbInt, b: AbInt)
-//   ensures (x == AbAdd(y, a)) && AbLt(a, b) ==> AbLt(x, AbAdd(y, b))
-
+lemma Props_all_nonneg ()
+  ensures forall x :: AbLt(int2adt(0), x) || x == int2adt(0)
+lemma Props_one_in_bound ()
+  ensures forall a, x :: (AbLt(a, x) || a == x) && (AbLt(x, AbAdd(a, int2adt(1)))) ==> a == x
 lemma Props_two_is_one_plus_one ()
   ensures int2adt(2) == AbAdd(int2adt(1), int2adt(1))
-lemma Props_plus_commutative ()
-  ensures forall x, y :: AbAdd(x, y) == AbAdd(y, x);
-lemma Props_plus_associative ()
-  ensures forall x, y, z :: AbAdd(AbAdd(x, y), z) == AbAdd(x, AbAdd(y, z))
-lemma Props_plus_pos_is_lt ()
-  ensures forall x, a :: AbPos(a) ==> AbLt(x, AbAdd(x, a));
-lemma Props_plus_and_minus ()
-  ensures forall x, y, z :: AbAdd(x, y) == z ==> AbSub(z, y) == x && AbSub(z, x) == y
-lemma Props_unfold_int2adt (i: nat)
-  ensures i == 0 ==> int2adt(i) == int2adt(0)
-  ensures i != 0 ==> int2adt(i) == AbAdd(int2adt(1), int2adt(i-1))
+lemma Props_gtzero_is_geqone ()
+  ensures forall x :: AbLt(int2adt(0), x) <==> AbLt(int2adt(1), x) || x == int2adt(1)
+lemma Props_gtzero_is_geqone_param (x: AbInt)
+  ensures AbLt(int2adt(0), x) <==> AbLt(int2adt(1), x) || x == int2adt(1)
 
-function method Length(xs: List): AbInt
+lemma Props_lt_is_not_geq () // x < y <==> !x > y && x != y
+  ensures forall x, y :: AbLt(x, y) <==> !(AbLt(y, x) || x == y)
+lemma Props_lt_addition () // a < b ==> x + a < x + b
+  ensures forall x, a, b:: AbLt(a, b) ==> AbLt(AbAdd(x, a), AbAdd(x, b))
+lemma Props_lt_transitive () // x < y < z
+  ensures forall x, y, z :: AbLt(x, y) && AbLt(y, z) ==> AbLt(x, z)
+lemma Props_lt_add_is_lt () // x + a < y ==> x < y
+  ensures forall x, y, a :: AbLt(AbAdd(x, a), y) ==> AbLt(x, y)
+
+lemma Props_add_commutative () // x + y == y + x
+  ensures forall x, y :: AbAdd(x, y) == AbAdd(y, x);
+lemma Props_add_associative () // (x + y) + z == x + (y + z)
+  ensures forall x, y, z :: AbAdd(AbAdd(x, y), z) == AbAdd(x, AbAdd(y, z))
+lemma Props_add_addition () // x + a == y + a ==> x == y
+  ensures forall x, y, a :: AbAdd(x, a) == AbAdd(y, a) <==> x == y
+lemma Props_add_identity () // x + 0 == 0 + x == x
+  ensures forall x :: AbAdd(x, int2adt(0)) == AbAdd(int2adt(0), x) == x
+
+lemma Props_add_less_is_lt () // x = y + a && a < b ==> x < y + b
+  ensures forall x, y, a, b :: (x == AbAdd(y, a)) && AbLt(a, b) ==> AbLt(x, AbAdd(y, b))
+// Some instantiation
+lemma Props_add_less_is_lt_param (x: AbInt, y: AbInt, a: AbInt, b: AbInt)
+  // Props_add_less_is_lt_param(s, n, int2adt(llen), int2adt(len));
+  ensures (x == AbAdd(y, a)) && AbLt(a, b) ==> AbLt(x, AbAdd(y, b))
+
+lemma Props_add_is_leq () //  x + a == y ==> x < y || x == y
+  ensures forall x, y, a :: (AbAdd(x, a) == y) ==> AbLt(x, y) || x == y
+lemma Props_add_pos_is_neq () // x + Positive != x
+  ensures forall x, a :: AbPos(a) ==> AbAdd(x, a) != x
+lemma Props_add_pos_is_pos () // x + Positive is Positive
+  ensures forall x, a :: AbPos(a) ==> AbPos(AbAdd(x, a)) 
+lemma Props_add_pos_is_lt () // x < x + Positive
+  ensures forall x, a :: AbPos(a) ==> AbLt(x, AbAdd(x, a));
+lemma Props_add2sub () // x + y == z ==> x = z - y && y = z - x
+  ensures forall x, y, z :: AbAdd(x, y) == z ==> AbSub(z, y) == x && AbSub(z, x) == y
+
+lemma Props_add_sub_is_add () // x + j + (i - j) == x + i
+    ensures forall x, i, j :: AbAdd(AbAdd(x, j), AbSub(i, j)) == AbAdd(x, i) // trigger may loop
+    // ensures forall x: AbInt, i, j, k: int :: k == i - j ==> AbAdd(AbAdd(x, int2adt(j)), int2adt(k)) == AbAdd(x, int2adt(i))
+// Some instantiation
+lemma Props_add_sub_is_add_param(x: AbInt, i: AbInt, j: AbInt)
+  // Props_add_sub_is_add_param(n, len, llen);
+  ensures AbAdd(AbAdd(x, j), AbSub(i, j)) == AbAdd(x, i)
+
+lemma Props_div_pos_is_pos () // Positive / 2 is Positive
+  ensures forall x :: AbPos(x) <==> AbPos(AbDiv2(x))
+lemma Props_div_add_leq_is_leq () // y <= x ==> (x+y)/2 <= x
+  ensures forall x, y :: AbLt(y, x) || x == y ==> AbLt(AbDiv2(AbAdd(x, y)), x) || AbDiv2(AbAdd(x, y)) == x
+lemma Props_div_add_leq_is_leq_param (x: AbInt, y: AbInt)
+  ensures AbLt(y, x) || x == y ==> AbLt(AbDiv2(AbAdd(x, y)), x) || AbDiv2(AbAdd(x, y)) == x
+lemma Props_div_addone_lt ()
+  ensures forall x :: AbLt(AbAdd(AbDiv2(x), int2adt(1)), x)
+
+// lemma Props_unfold_int2adt (i: nat)
+//   ensures i == 0 ==> int2adt(i) == int2adt(0)
+//   ensures i != 0 ==> int2adt(i) == AbAdd(int2adt(1), int2adt(i-1))
+
+function method Length(xs: List<AbInt>): AbInt
 {
   match xs
   case Nil => int2adt(0)
-  case Cons(_, tail) => AbAdd(int2adt(1), Length(tail))
+  case Cons(_, tail) =>  AbAdd(int2adt(1), Length(tail))
 }
-
-function method SmallestMissingNumber(xs: List<AbInt>): AbInt
-{
-  SMN(xs, int2adt(0), Length(xs))
-}
-
-function method SMN(xs: List<AbInt>, n: AbInt, len: AbInt): AbInt
-  requires len == Length(xs)
-  decreases adt2int(Length(xs))
-{
-  Props_two_is_one_plus_one ();
-  Props_plus_commutative ();
-  Props_plus_and_minus ();
-  if AbLt(int2adt(2), len) || int2adt(2) == len then
-    var (L, R) := Split(xs, AbAdd(n, AbDiv2(len)));
-    var llen := Length(L);
-    if AbLt(llen, AbDiv2(len)) then
-      SMN(L, n, llen)
-    else
-      SMN(R, AbAdd(n, llen), AbSub(len, llen))
-  else if xs.Cons? then
-    if xs.head == n then AbAdd(n, int2adt(1)) else n
-  else
-    n
-}
-
-function method SMN'(xs: List<AbInt>, n: AbInt, len: AbInt): AbInt
-  requires len == Length(xs)
-  // decreases adt2int(Length(xs))
-{
-  Props_two_is_one_plus_one ();
-  Props_plus_commutative ();
-  Props_plus_and_minus ();
-  if xs == Nil then
-    n
-  else
-    var half := AbDiv2(AbAdd(len, int2adt(1)));
-    var (L, R) := Split(xs, AbAdd(n, half));
-    var llen := Length(L);
-    if AbLt(llen, half) then
-      SMN'(L, n, llen)
-    else
-      SMN'(R, AbAdd(n, llen), AbSub(len, llen))
-}
-
-function method SMN''(xs: List<AbInt>, n: AbInt, len: AbInt): AbInt
-  requires len == Length(xs)
-  decreases xs
-{
-  Props_two_is_one_plus_one ();
-  Props_plus_commutative ();
-  Props_plus_and_minus ();
-  if xs == Nil then
-    n
-  else
-    var half := AbAdd(AbDiv2(len), int2adt(1));
-    var (L, R) := Split(xs, AbAdd(n, half));
-    var llen := Length(L);
-    if AbLt(llen, half) then
-      SMN''(L, n, llen)
-    else
-      SMN''(R, AbAdd(n, llen), AbSub(len, llen))
-}
-
+ 
 function method Split(xs: List<AbInt>, b: AbInt): (List<AbInt>, List<AbInt>)
   ensures var r := Split(xs, b); Length(xs) == AbAdd(Length(r.0), Length(r.1))
   decreases xs
 {
-  Props ();
-  Props_plus_commutative ();
-  Props_plus_associative ();
+  Props_add_commutative ();
+  Props_add_associative ();
+  Props_add_identity ();
   match xs
   case Nil => (Nil, Nil)
   case Cons(x, tail) =>
@@ -211,21 +178,23 @@ lemma Split_Correct(xs: List<AbInt>, b: AbInt)
     Split_Correct(tail, b);
 }
 
-function Elements(xs: List): set
+function Elements(xs: List<AbInt>): set<AbInt>
 {
   match xs
   case Nil => {}
   case Cons(x, tail) => {x} + Elements(tail)
 }
 
-lemma Elements_Property(xs: List)
+lemma Elements_Property(xs: List<AbInt>)
   requires NoDuplicates(xs)
-  ensures int2adt(|Elements(xs)|) == Length(xs)
+  ensures AbSetLen(Elements(xs)) == Length(xs)
 {
-  Props_unfold_int2adt(|Elements(xs)|);
+  SetLen_Props();
+  Props_add_commutative ();
+  Props_add_associative ();
 }
 
-predicate NoDuplicates(xs: List)
+predicate NoDuplicates(xs: List<AbInt>)
 {
   match xs
   case Nil => true
@@ -235,20 +204,27 @@ predicate NoDuplicates(xs: List)
 
 // standard theorems and their proofs
 
-lemma Cardinality(A: set, B: set)
+lemma Cardinality(A: set<AbInt>, B: set<AbInt>)
   requires A <= B
-  ensures |A| <= |B|
+  ensures AbLt(AbSetLen(A), AbSetLen(B)) || AbSetLen(A) == AbSetLen(B)
 {
+  SetLen_Props ();
+  Props_all_nonneg ();
+  Props_add_addition ();
+  Props_add_commutative ();
+  Props_lt_addition ();
   if A != {} {
     var x :| x in A;
     Cardinality(A - {x}, B - {x});
   }
 }
 
-lemma SetEquality(A: set, B: set)
-  requires A <= B && |A| == |B|
+lemma SetEquality(A: set<AbInt>, B: set<AbInt>)
+  requires A <= B && AbSetLen(A) == AbSetLen(B)
   ensures A == B
 {
+  SetLen_Props ();
+  Props_add_addition ();
   if A == {} {
   } else {
     var x :| x in A;
@@ -257,7 +233,7 @@ lemma SetEquality(A: set, B: set)
 }
 
 function IntRange(lo: AbInt, len: AbInt): set<AbInt>
-  ensures int2adt(|IntRange(lo, len)|) == len
+  ensures AbSetLen(IntRange(lo, len)) == len
 {
   var S := AbBoundSet(lo, len);
   // assume AbLt(int2adt(len - 1), int2adt(len));
@@ -267,179 +243,301 @@ function IntRange(lo: AbInt, len: AbInt): set<AbInt>
   S
 }
 
-// // proof of lemmas supporting proof of main theorem
+function method SmallestMissingNumber(xs: List<AbInt>): AbInt
+{
+  SMN(xs, int2adt(0), Length(xs))
+}
 
-// lemma SmallestMissingNumber_Correct(xs: List<AbInt>)
-//   requires NoDuplicates(xs)
-//   ensures var s := SmallestMissingNumber(xs);
-//     s !in Elements(xs) &&
-//     forall x :: (AbLt(int2adt(0), x) || int2adt(0) == x) && AbLt(x, s) ==> x in Elements(xs)
-// {
-//   Props ();
-//   SMN_Correct(xs, int2adt(0), Length(xs));
-// }
+function method SMN(xs: List<AbInt>, n: AbInt, len: AbInt): AbInt
+  requires len == Length(xs)
+  decreases adt2dt(len)
+{
+  Props_add_commutative ();
+  if AbLt(int2adt(2), len) || int2adt(2) == len then
+    var (L, R) := Split(xs, AbAdd(n, AbDiv2(len)));
+    var llen := Length(L);
+    Props_all_nonneg ();
+    Props_lt_is_not_geq ();
+    Props_int_pos(2); // AbInt0 < AbInt2
+    Props_add_pos_is_lt ();
+    if AbLt(llen, AbDiv2(len)) then
+      Props_lt_transitive (); // AbInt0 < len
+      Props_lt_add_is_lt ();
+      Props_adt_dt_lt (llen, len);
+      SMN(L, n, llen)
+    else
+      Props_div_pos_is_pos ();
+      Props_add2sub ();
+      Props_adt_dt_lt (AbSub(len, llen), len);
+      SMN(R, AbAdd(n, llen), AbSub(len, llen))
+  else if xs.Cons? then
+    if xs.head == n then AbAdd(n, int2adt(1)) else n
+  else
+    n
+}
 
-// // element, len, index -> abstract type
-// lemma SMN_Correct(xs: List<AbInt>, n: AbInt, len: AbInt)
-//   requires NoDuplicates(xs)
-//   requires forall x :: x in Elements(xs) ==> (AbLt(n, x) || n == x)
-//   requires len == Length(xs)
-//   ensures var s := SMN(xs, n, len);
-//     (AbLt(n, s) || n == s) &&
-//     (AbLt(s, AbAdd(n, len)) || s == AbAdd(n, len)) &&
-//     s !in Elements(xs) &&
-//     forall x ::(AbLt(n, x) || n == x) && AbLt(x, s) ==> x in Elements(xs)
-//   decreases len
-// {
-//   Props ();
-//   // Props_two_is_one_plus_one ();
-//   // Props_plus_commutative ();
-//   // Props_plus_and_minus ();
-//   if AbLt(int2adt(2), len) || int2adt(2) == len {
-//     var (L, R) := Split(xs, AbAdd(n, AbDiv2(len)));
-//     Split_Correct(xs, AbAdd(n, AbDiv2(len)));
-//     var llen := Length(L);
-//     Elements_Property(L);  // NoDuplicates property
-//     var bound := IntRange(n, AbDiv2(len));
-//     // Props_lt_is_not_geq ();
-//     Cardinality(Elements(L), bound);
-//     if AbLt(llen, AbDiv2(len)) {
-//       var s := SMN(L, n, llen);
-//       SMN_Correct(L, n, llen);
-//       // Props_lt_addition (); // Lt(s, n+llen) ==> Lt(s, n+len)
-//       // Props_lt_transitive ();
-//       // Props_eq_less_is_lt (); // s==n+llen ==> Lt(s, n+len)
-//       // Note: instantiation for no trigger loop
-//       Props_eq_less_is_lt_param(s, n, llen, len);
-//     } else {
-//       var s := SMN(R, AbAdd(n, llen), AbSub(len, llen));
-//       SMN_Correct(R, AbAdd(n, llen), AbSub(len, llen));
-//       // Props_plus_lt_is_lt (); // Lt(n+llen, s) ==> Lt(n, s)      
-//       // Props_plus_is_leq (); // n+llen == s ==> Lt(n, s)
-//       // Props_plus_minus_is_eq();
-//       // Note: instantiation for no trigger loop
-//       Props_plus_minus_is_eq_param(n, len, llen);
-//       forall x | (AbLt(n, x) || n == x) && AbLt(x, s)
-//         ensures x in Elements(xs)
-//       {
-//         if AbLt(x, AbAdd(n, llen)) {
-//           SetEquality(Elements(L), bound);
-//         }
-//       }
-//     }
-//   } 
-//   else {
-//     Props_int_pos(1);
-//     // Props_plus_is_leq ();
-//     // Props_plus_pos_is_neq ();
-//     // Props_one_in_bound ();
-//     // Props_lt_is_not_geq ();
-//     // Props_plus_zero ();
-//   }
-// }
+// proof of lemmas supporting proof of main theorem
 
-// lemma SMN'_Correct(xs: List<AbInt>, n: AbInt, len: nat)
-//   requires NoDuplicates(xs)
-//   requires forall x :: x in Elements(xs) ==> (AbLt(n, x) || n == x)
-//   requires len == Length(xs)
-//   ensures var s := SMN'(xs, n, len);
-//     (AbLt(n, s) || n == s) &&
-//     (AbLt(s, AbAdd(n, int2adt(len))) || s == AbAdd(n, int2adt(len))) &&
-//     s !in Elements(xs) &&
-//     forall x :: (AbLt(n, x) || n == x) && AbLt(x, s) ==> x in Elements(xs)
-//   decreases len
-// { 
-//   Props ();
-//   if xs == Nil {
-//   } else {
-//     var half := (len + 1) / 2;
-//     var (L, R) := Split(xs, AbAdd(n, int2adt(half)));
-//     Split_Correct(xs, AbAdd(n, int2adt(half)));
-//     var llen := Length(L);
-//     Elements_Property(L);  // use the NoDuplicates property
-//     var bound := IntRange(n, half);
-//     Cardinality(Elements(L), bound);
-//     if llen < half {
-//       var s := SMN'(L, n, llen);
-//       SMN'_Correct(L, n, llen);
-//       Props_int_cmp_lt(llen, half);
-//       Props_int_cmp_lt(llen, len);
-//       // Note: instantiation for no trigger loop
-//       Props_eq_less_is_lt_param(s, n, int2adt(llen), int2adt(len));
-//     } else {
-//       var s := SMN'(R, AbAdd(n, int2adt(llen)), len - llen);
-//       SMN'_Correct(R, AbAdd(n, int2adt(llen)), len - llen);
-//       // Note: instantiation for no trigger loop
-//       Props_plus_minus_is_eq_param(n, len, llen);
-//       forall x | (AbLt(n, x) || n == x) && AbLt(x, s)
-//         ensures x in Elements(xs)
-//       {
-//         if AbLt(x, AbAdd(n, int2adt(llen))) {
-//           SetEquality(Elements(L), bound);
-//         }
-//       }
-//     }
-//   }
-// }
+lemma SmallestMissingNumber_Correct(xs: List<AbInt>)
+  requires NoDuplicates(xs)
+  ensures var s := SmallestMissingNumber(xs);
+    s !in Elements(xs) &&
+    forall x :: (AbLt(int2adt(0), x) || int2adt(0) == x) && AbLt(x, s) ==> x in Elements(xs)
+{
+  Props_all_nonneg ();
+  SMN_Correct(xs, int2adt(0), Length(xs));
+}
 
-// lemma SMN''_Correct(xs: List<AbInt>, n: AbInt, len: nat)
-//   requires NoDuplicates(xs)
-//   requires forall x :: x in Elements(xs) ==> (AbLt(n, x) || n == x)
-//   requires len == Length(xs)
-//   ensures var s := SMN''(xs, n, len);
-//     (AbLt(n, s) || n == s) &&
-//     (AbLt(s, AbAdd(n, int2adt(len))) || s == AbAdd(n, int2adt(len))) &&
-//     s !in Elements(xs) &&
-//     forall x :: (AbLt(n, x) || n == x) && AbLt(x, s) ==> x in Elements(xs)
-//   decreases len
-// {
-//   Props ();
-//   if xs == Nil {
-//   } else {
-//     var half := len / 2 + 1;
-//     var (L, R) := Split(xs, AbAdd(n, int2adt(half)));
-//     Split_Correct(xs, AbAdd(n, int2adt(half)));
-//     var llen := Length(L);
-//     Elements_Property(L);  // use the NoDuplicates property
-//     var bound := IntRange(n, half);
-//     Cardinality(Elements(L), bound);
-//     if llen < half {
-//       var s := SMN''(L, n, llen);
-//       SMN''_Correct(L, n, llen);
-//       Props_int_cmp_lt(llen, half);
-//       Props_int_cmp_lt(llen, len);
-//       // Note: instantiation for no trigger loop
-//       Props_eq_less_is_lt_param(s, n, int2adt(llen), int2adt(len));
-//     } else {
-//       var s := SMN''(R, AbAdd(n, int2adt(llen)), len - llen);
-//       SMN''_Correct(R, AbAdd(n, int2adt(llen)), len - llen);
-//       // Note: instantiation for no trigger loop
-//       Props_plus_minus_is_eq_param(n, len, llen);
-//       forall x | (AbLt(n, x) || n == x) && AbLt(x, s)
-//         ensures x in Elements(xs)
-//       {
-//         if AbLt(x, AbAdd(n, int2adt(llen))) {
-//           SetEquality(Elements(L), bound);
-//         }
-//       }
-//     }
-//   }
-// }
+// element, len, index -> abstract type
+lemma SMN_Correct(xs: List<AbInt>, n: AbInt, len: AbInt)
+  requires NoDuplicates(xs)
+  requires forall x :: x in Elements(xs) ==> (AbLt(n, x) || n == x)
+  requires len == Length(xs)
+  ensures var s := SMN(xs, n, len);
+    (AbLt(n, s) || n == s) &&
+    (AbLt(s, AbAdd(n, len)) || s == AbAdd(n, len)) &&
+    s !in Elements(xs) &&
+    forall x ::(AbLt(n, x) || n == x) && AbLt(x, s) ==> x in Elements(xs)
+  decreases adt2dt(len)
+{
+  Props_add_commutative (); // x + y = y + x
+  Props_all_nonneg ();
+  Props_lt_is_not_geq (); // x < y <==> !x > y && x != y
+  if AbLt(int2adt(2), len) || int2adt(2) == len {
+    var (L, R) := Split(xs, AbAdd(n, AbDiv2(len)));
+    Split_Correct(xs, AbAdd(n, AbDiv2(len)));
+    var llen := Length(L);
+    Elements_Property(L);  // NoDuplicates property
+    var bound := IntRange(n, AbDiv2(len));
+    Cardinality(Elements(L), bound);
+    Props_int_pos(2); // 0 < 2
+    Props_div_pos_is_pos ();
+    Props_add_pos_is_lt (); // x < x + Positive
+    Props_lt_add_is_lt (); // x + Postive < y ==> x < y
+    if AbLt(llen, AbDiv2(len)) {
+      var s := SMN(L, n, llen);
+      Props_lt_transitive (); // x < y < z      
+      Props_adt_dt_lt (llen, len); // decreases (pre: llen < len/2 < len)
+      SMN_Correct(L, n, llen);
+      Props_lt_addition (); // a < b ==> x + a < x + b: Lt(s, n+llen) ==> Lt(s, n+len)
+      // Props_add_less_is_lt ();  // x = y + a && a < b ==> x < y + b: s==n+llen ==> Lt(s, n+len)
+      Props_add_less_is_lt_param(s, n, llen, len); // no trigger loop
+    } else {
+      Props_add2sub ();
+      Props_adt_dt_lt (AbSub(len, llen), len);
+      var s := SMN(R, AbAdd(n, llen), AbSub(len, llen));
+      SMN_Correct(R, AbAdd(n, llen), AbSub(len, llen));
+      Props_add_is_leq (); // x + a == y ==> x < y || x == y: n+llen == s ==> Lt(n, s)
+      // Props_add_sub_is_add();
+      Props_add_sub_is_add_param(n, len, llen); // no trigger loop
+      forall x | (AbLt(n, x) || n == x) && AbLt(x, s)
+        ensures x in Elements(xs)
+      {
+        if AbLt(x, AbAdd(n, llen)) {
+          SetEquality(Elements(L), bound);
+        }
+      }
+    }
+  } 
+  else {
+    Props_int_pos(1); // 0 < 1
+    Props_two_is_one_plus_one ();
+    Props_one_in_bound ();
+    Props_add_identity ();
+    Props_add_addition ();
+    Props_add_pos_is_neq (); // x + Positive != x
+    Props_add_is_leq (); // x + a == y ==> x < y || x == y
+    Props_add_pos_is_pos (); // x + Positive = Positive
+  }
+}
+
+function method SMN'(xs: List<AbInt>, n: AbInt, len: AbInt): AbInt
+  requires len == Length(xs)
+  decreases adt2dt(len)
+{
+  if xs == Nil then n
+  else
+    var half := AbDiv2(AbAdd(len, int2adt(1))); // half = (len+1)/2
+    var (L, R) := Split(xs, AbAdd(n, half));
+    var llen := Length(L);
+    Props_int_pos(1); // 0 < 1
+    Props_all_nonneg ();
+    // Props_add_identity ();
+    Props_add_pos_is_pos (); // x + Positive = Positive
+    Props_add_pos_is_lt (); // x < x + Positive
+    Props_gtzero_is_geqone_param (len); // x > 0 ==> x >= 1
+    Props_add_commutative ();
+    Props_lt_transitive ();
+    Props_div_add_leq_is_leq_param (len, int2adt(1));  // no trigger loop
+    if AbLt(llen, half) then
+      Props_adt_dt_lt (llen, len);
+      SMN'(L, n, llen)
+    else
+      Props_add2sub ();
+      Props_lt_is_not_geq ();
+      Props_div_pos_is_pos ();
+      Props_adt_dt_lt (AbSub(len, llen), len);
+      SMN'(R, AbAdd(n, llen), AbSub(len, llen))
+}
+
+lemma SMN'_Correct(xs: List<AbInt>, n: AbInt, len: AbInt)
+  requires NoDuplicates(xs)
+  requires forall x :: x in Elements(xs) ==> (AbLt(n, x) || n == x)
+  requires len == Length(xs)
+  ensures var s := SMN'(xs, n, len);
+    (AbLt(n, s) || n == s) &&
+    (AbLt(s, AbAdd(n, len)) || s == AbAdd(n, len)) &&
+    s !in Elements(xs) &&
+    forall x ::(AbLt(n, x) || n == x) && AbLt(x, s) ==> x in Elements(xs)
+  decreases adt2dt(len)
+{
+  Props_lt_is_not_geq (); // x < y <==> !x > y && x != y
+  Props_add_identity ();
+  if xs == Nil {
+  } else {
+    var half := AbDiv2(AbAdd(len, int2adt(1))); // half = (len+1)/2
+    var (L, R) := Split(xs, AbAdd(n, half));
+    Split_Correct(xs, AbAdd(n, half));
+    var llen := Length(L);
+    Elements_Property(L);  // use the NoDuplicates property
+    var bound := IntRange(n, half);
+    Cardinality(Elements(L), bound);
+    Props_int_pos(1); // 0 < 1
+    Props_all_nonneg ();
+    Props_add_pos_is_pos (); // x + Positive = Positive
+    Props_add_pos_is_lt (); // x < x + Positive
+    Props_gtzero_is_geqone_param (len); // x > 0 ==> x >= 1
+    Props_add_commutative ();
+    Props_lt_transitive ();
+    Props_div_add_leq_is_leq_param (len, int2adt(1));  // no trigger loop
+    if AbLt(llen, half) {
+      var s := SMN'(L, n, llen);
+      Props_adt_dt_lt (llen, len);
+      SMN'_Correct(L, n, llen);
+      Props_lt_addition ();
+      Props_add_less_is_lt_param(s, n, llen, len); // no trigger loop
+    } else {
+      Props_add2sub ();
+      Props_div_pos_is_pos ();
+      Props_adt_dt_lt (AbSub(len, llen), len);
+      var s := SMN'(R, AbAdd(n, llen), AbSub(len, llen));
+      SMN'_Correct(R, AbAdd(n, llen), AbSub(len, llen));
+      Props_add_sub_is_add_param(n, len, llen); // no trigger loop
+      forall x | (AbLt(n, x) || n == x) && AbLt(x, s)
+        ensures x in Elements(xs)
+      {
+        if AbLt(x, AbAdd(n, llen)) {
+          SetEquality(Elements(L), bound);
+        }
+      }
+    }
+  }
+}
+
+function method SMN''(xs: List<AbInt>, n: AbInt, len: AbInt): AbInt
+  requires len == Length(xs)
+  decreases adt2dt(len)
+{
+  if xs == Nil then n
+  else
+    var half := AbAdd(AbDiv2(len), int2adt(1)); // half = len/2 + 1
+    var (L, R) := Split(xs, AbAdd(n, half));
+    var llen := Length(L);
+    Props_int_pos(1); // 0 < 1
+    Props_all_nonneg ();
+    // Props_add_identity ();
+    Props_add_pos_is_pos (); // x + Positive = Positive
+    Props_add_pos_is_lt (); // x < x + Positive
+    Props_gtzero_is_geqone_param (len); // x > 0 ==> x >= 1
+    Props_add_commutative ();
+    Props_lt_transitive ();
+    Props_div_addone_lt ();
+    if AbLt(llen, half) then
+      Props_adt_dt_lt (llen, len);
+      SMN''(L, n, llen)
+    else
+      Props_add2sub ();
+      Props_lt_is_not_geq ();
+      Props_div_pos_is_pos ();
+      Props_adt_dt_lt (AbSub(len, llen), len);
+      SMN''(R, AbAdd(n, llen), AbSub(len, llen))
+}
+
+lemma SMN''_Correct(xs: List<AbInt>, n: AbInt, len: AbInt)
+  requires NoDuplicates(xs)
+  requires forall x :: x in Elements(xs) ==> (AbLt(n, x) || n == x)
+  requires len == Length(xs)
+  ensures var s := SMN''(xs, n, len);
+    (AbLt(n, s) || n == s) &&
+    (AbLt(s, AbAdd(n, len)) || s == AbAdd(n, len)) &&
+    s !in Elements(xs) &&
+    forall x ::(AbLt(n, x) || n == x) && AbLt(x, s) ==> x in Elements(xs)
+  decreases adt2dt(len)
+{
+  Props_lt_is_not_geq (); // x < y <==> !x > y && x != y
+  Props_add_identity ();
+  if xs == Nil {
+  } else {
+    var half := AbAdd(AbDiv2(len), int2adt(1)); // half = len/2 + 1
+    var (L, R) := Split(xs, AbAdd(n, half));
+    Split_Correct(xs, AbAdd(n, half));
+    var llen := Length(L);
+    Elements_Property(L);  // use the NoDuplicates property
+    var bound := IntRange(n, half);
+    Cardinality(Elements(L), bound);
+    Props_int_pos(1); // 0 < 1
+    Props_all_nonneg ();
+    Props_add_pos_is_pos (); // x + Positive = Positive
+    Props_add_pos_is_lt (); // x < x + Positive
+    Props_gtzero_is_geqone_param (len); // x > 0 ==> x >= 1
+    Props_add_commutative ();
+    Props_lt_transitive ();
+    Props_div_addone_lt ();
+    if AbLt(llen, half) {
+      var s := SMN''(L, n, llen);
+      Props_adt_dt_lt (llen, len);
+      SMN''_Correct(L, n, llen);
+      Props_lt_addition ();
+      Props_add_less_is_lt_param(s, n, llen, len); // no trigger loop
+    } else {
+      Props_add2sub ();
+      Props_div_pos_is_pos ();
+      Props_adt_dt_lt (AbSub(len, llen), len);
+      var s := SMN''(R, AbAdd(n, llen), AbSub(len, llen));
+      SMN''_Correct(R, AbAdd(n, llen), AbSub(len, llen));
+      Props_add_sub_is_add_param(n, len, llen); // no trigger loop
+      forall x | (AbLt(n, x) || n == x) && AbLt(x, s)
+        ensures x in Elements(xs)
+      {
+        if AbLt(x, AbAdd(n, llen)) {
+          SetEquality(Elements(L), bound);
+        }
+      }
+    }
+  }
+}
 
 // TODO: need more concrete props to make it verified.
 method Main() {
-  Props();
-  Props_plus_minus_is_eq ();
-
-  // Note: this assumption is wrong.
-  assume forall x, y, a :: (AbAdd(x, a) == y) && AbNonNeg(a) ==> AbLt(x, y);
-
   var xs := Nil;
+  assert Length(xs) == int2adt(0);
   var s := SmallestMissingNumber(xs);
+  Props_all_nonneg ();
+  Props_add_associative ();
+  Props_add_identity ();
+  Props_add_commutative ();
+  Props_add_pos_is_pos ();
+  Props_int_pos(2);
+  Props_lt_transitive ();
+  Props_lt_is_not_geq ();
   assert s == int2adt(0);
   print s, " ";  // 0
   var a := Cons(int2adt(2), Cons(int2adt(0), Nil));
-  // assert SmallestMissingNumber(a) == int2adt(1);
+  Props_two_is_one_plus_one ();
+  assume int2adt(1) == AbDiv2(int2adt(2));
+  assume AbLt(int2adt(0), int2adt(1));
+  assume AbLt(int2adt(1), int2adt(2));
+  // assert SmallestMissingNumbxer(a) == int2adt(1);
   // print SmallestMissingNumber(a), " ";  // 1
   a := Cons(int2adt(3), Cons(int2adt(1), a));
   // assert SmallestMissingNumber(a) == int2adt(4);
